Para o alongamento quadr√°tico:
\[\varepsilon_q=\frac{1}{2}(\lambda^2-1)\]
\[\lambda^2=1+2\varepsilon_q\]
\[\lambda=\sqrt{1+2\varepsilon_q}\]
\[\lambda(\hat{\utilde{\mathbf{m}}}^r)=\sqrt{1+2(\hat{\utilde{\mathbf{m}}}^r\cdot\underline{\mathbf{E}}\hat{\utilde{\mathbf{m}}}^r)}\]

Para o alongamento linear:
\[\varepsilon_l=\lambda-1\]
\[\varepsilon_l(\hat{\utilde{\mathbf{m}}}^r)=\sqrt{1+2(\hat{\utilde{\mathbf{m}}}^r\cdot\underline{\mathbf{E}}\hat{\utilde{\mathbf{m}}}^r)}-1\]
\[\varepsilon_l(\hat{\utilde{\mathbf{m}}}^r)=\sqrt{1+2\varepsilon_q}-1\]